DeepWiki/SymbolicIntegration/ComputableTowerWellFounded.lean
@@ -1,6 +1,7 @@
 import DeepWiki.SymbolicIntegration.ComputableTowerGcdFFCore
 import DeepWiki.SymbolicIntegration.ComputableTowerIntegrate
 import DeepWiki.SymbolicIntegration.ComputableWellFounded
+import DeepWiki.SymbolicIntegration.ComputableWellFoundedDioph
 import DeepWiki.SymbolicIntegration.ComputableWellFounded2
 import DeepWiki.SymbolicIntegration.ComputableWellFounded3
 import DeepWiki.SymbolicIntegration.ComputableWellFounded4
